src/cddl/test/dpe/CDDLTest.DPE.CertifyKeyOutput.fst
@@ -1,0 +1,256 @@
+module CDDLTest.DPE.CertifyKeyOutput
+module EqTest = CDDL.Spec.EqTest
+open CDDLTest.Test
+open Pulse.Lib
+open Pulse.Lib.Pervasives
+open CDDLTest.Destructors
+#lang-pulse
+open CDDL.Pulse.Parse.Base
+module S = Pulse.Lib.Slice
+module U8 = FStar.UInt8
+open CDDL.Pulse.Types
+module T = CDDL.Pulse.AST.Tactics
+open CDDL.Pulse.AST.Bundle
+open CBOR.Spec.API.Type
+open CDDL.Spec.Base
+open CDDLTest.DPE.Common
+
+let pretty_bytes (x:Seq.seq UInt8.t) =
+  spect_evercddl_bytes_pretty_right (spect_evercddl_bstr_pretty_right x)
+
+let _ = rel_evercddl_certifykeyoutputargs
+
+
+let struct_has_pubkey_and_cert (hres:spect_evercddl_certifykeyoutputargs_pretty) (pk cert:Seq.seq UInt8.t) =
+  hres._x0 == Some (pretty_bytes pk) /\
+  hres._x1 == Some (pretty_bytes cert) /\
+  hres._x2 == None
+
+let of_bytes (#p:perm) (x:evercddl_bytes_pretty) (s:Slice.slice UInt8.t) =
+  let x = evercddl_bstr_pretty_left (evercddl_bytes_pretty_left x) in
+  x.s == s /\
+  x.p == p
+
+let of_bytes_option #p (x:option evercddl_bytes_pretty) (s:option (Slice.slice UInt8.t)) =
+  match x, s with
+  | None, None -> True
+  | Some x, Some s -> of_bytes #p x s
+  | _ -> False
+
+fn mk_evercddl_bytes_pretty
+    (x:Slice.slice UInt8.t)
+    (#p #w:erased _)
+requires
+  pts_to x #p w
+returns res:_
+ensures
+  rel_option rel_evercddl_bytes res (Some <| pretty_bytes w) **
+  pure (of_bytes_option #p res (Some x))
+{
+  admit()
+}
+
+fn mk_evercddl_bytes_pretty_none ()
+requires emp
+ensures
+  rel_option rel_evercddl_bytes None None
+{
+  admit()
+}
+
+// ghost
+// fn mk_rel_pair #a0 #b0 #a1 #b1 (r1:rel a0 b0) (r1:rel a1 b1)
+// requires
+//    r0 x0 y0 ** r1 x1 y1
+// ensures
+
+//     (x:Slice.slice UInt8.t)
+//     (#p #w:erased _)
+// requires
+//   pts_to x #p w
+// returns res:_
+// ensures
+//   rel_option rel_evercddl_bytes res (Some <| pretty_bytes w)
+// {
+//   admit()
+// }
+
+
+fn mk_tstr_any_empty ()
+requires emp
+returns res:_
+ensures exists* w. tstr_any res w
+{
+  admit()
+}
+
+[@@pulse_unfold]
+unfold
+let my_unfold_l (#a:Type) (s:list string) (p:a) = norm [delta_only s; hnf; iota; primops] p
+
+ghost
+fn fold_l (s:list string) (p:slprop)
+requires my_unfold_l s p
+ensures p
+{
+  norm_spec [delta_only s; hnf; iota; primops] p;
+  rewrite each (my_unfold_l s p) as p;
+}
+
+ghost
+fn unfold_l (s:list string) (p:slprop)
+requires p
+ensures my_unfold_l s p
+{
+  norm_spec [delta_only s; hnf; iota; primops] p;
+  rewrite each p as (my_unfold_l s p);
+}
+
+ghost
+fn mk_rel_pair (#a0 #b0 #a1 #b1:Type0) (r0:rel a0 b0) (r1:rel a1 b1) (x0:a0) (#y0:b0) (x1:a1) (#y1:b1)
+requires
+  r0 x0 y0 ** r1 x1 y1
+ensures
+  rel_pair r0 r1 (x0, x1) (y0, y1)
+{
+  rewrite (r0 x0 y0 ** r1 x1 y1)
+  as (rel_pair r0 r1 (x0, x1) (y0, y1));
+}
+
+fn fold_certify_key_output_args (x:_) (w:erased _)
+requires
+  rel_pair (rel_pair (rel_option rel_evercddl_bytes) (rel_option rel_evercddl_bytes))
+           (rel_option rel_evercddl_bytes)
+          x w
+returns res:_
+ensures exists* (hres:spect_evercddl_certifykeyoutputargs_pretty).
+      rel_evercddl_certifykeyoutputargs res hres **
+      pure (hres._x0 == (fst (fst w)) /\
+            hres._x1 == (snd (fst w)) /\
+            hres._x2 == snd w /\
+            res.intkey1 ==  (fst (fst x)) /\
+            res.intkey2 ==  (snd (fst x)) /\
+            res.intkey3 == None)
+{
+  admit()
+}
+
+let res_has_pk_and_cert (res:evercddl_certifykeyoutputargs_pretty) (pk cert:Slice.slice UInt8.t) p q =
+  of_bytes_option #p res.intkey1 (Some pk) /\
+  of_bytes_option #q res.intkey2 (Some cert) /\
+  of_bytes_option #q res.intkey3 None
+
+fn write_certify_key_output
+    (pubkey:Slice.slice UInt8.t)
+    (cert:Slice.slice UInt8.t)
+    (#pk #c:erased _) (#p #q:perm)
+requires
+    pts_to pubkey #p pk **
+    pts_to cert #q c
+returns res:_
+ensures
+  exists* hres. 
+    rel_evercddl_certifykeyoutputargs res hres **
+    pure (struct_has_pubkey_and_cert hres pk c /\ 
+          res_has_pk_and_cert res pubkey cert p q)
+{
+  let pk = mk_evercddl_bytes_pretty pubkey;
+  let cert = mk_evercddl_bytes_pretty cert;
+  mk_rel_pair (rel_option rel_evercddl_bytes) (rel_option rel_evercddl_bytes) pk cert;
+  mk_evercddl_bytes_pretty_none ();
+  mk_rel_pair (rel_pair (rel_option rel_evercddl_bytes) (rel_option rel_evercddl_bytes)) (rel_option rel_evercddl_bytes) _ None;
+  let res = fold_certify_key_output_args _ _;
+  res
+}
+ 
+let is_serialized_certify_key_output hres w =
+  exists sz.
+    impl_serialize_post (coerce_spec bundle_certifykeyoutputargs
+                .b_spec
+              spect_evercddl_certifykeyoutputargs_pretty
+              ())
+          hres
+          w
+          sz
+
+fn write_certify_key_output_main
+    (out:Slice.slice UInt8.t)
+    (pubkey:Slice.slice UInt8.t)
+    (cert:Slice.slice UInt8.t)
+    (#pk #c:erased _) (#p #q:perm)
+requires
+  exists* w.
+    pts_to pubkey #p pk **
+    pts_to cert #q c **
+    pts_to out w
+returns res:(_ & bool)
+ensures
+  exists* hres w.
+    rel_evercddl_certifykeyoutputargs (fst res) hres **
+    pts_to out w **
+    pure (struct_has_pubkey_and_cert hres pk c /\
+          res_has_pk_and_cert (fst res) pubkey cert p q) **
+    pure (snd res ==>  is_serialized_certify_key_output hres w)
+{
+  let res = write_certify_key_output pubkey cert;
+  let sz = serialize_certifykeyoutputargs' _ out;
+  if (sz = 0sz) {
+    (res, false)
+  }
+  else {
+    (res, true)
+  }
+}
+
+ghost
+fn destruct_certifykeyoutputargs x hres pubkey cert p q pk c
+requires
+    rel_evercddl_certifykeyoutputargs x hres **
+    pure (of_bytes_option #p x.intkey1 (Some pubkey) /\
+          of_bytes_option #q x.intkey2 (Some cert) /\
+          of_bytes_option #q x.intkey3 None /\
+          struct_has_pubkey_and_cert hres pk c)
+ensures
+    pts_to pubkey #p pk **
+    pts_to cert #q c
+{
+  slprop_equivs();
+  unfold (rel_evercddl_certifykeyoutputargs x hres);
+  destruct_rel_fun _ _ _ _ _;
+  drop_ (Trade.trade _ _);
+  destruct_pair _ _ ((evercddl_certifykeyoutputargs_pretty_left x)) _ ();
+  drop_ (Trade.trade _ _);
+  destruct_pair (rel_option rel_evercddl_bytes) (rel_option rel_evercddl_bytes) (fst (evercddl_certifykeyoutputargs_pretty_left x)) (fst (spect_evercddl_certifykeyoutputargs_pretty_left hres)) ();
+  show_proof_state;
+}
+
+fn write_certify_key_output_alt
+    (out:Slice.slice UInt8.t)
+    (pubkey:Slice.slice UInt8.t)
+    (cert:Slice.slice UInt8.t)
+    (#pk #c:erased _) (#p #q:perm)
+requires
+  exists* w.
+    pts_to pubkey #p pk **
+    pts_to cert #q c **
+    pts_to out w
+returns res:bool
+ensures
+  exists* w.
+    pts_to pubkey #p pk **
+    pts_to cert #q c **
+    pts_to out w **
+    pure (exists hres. res ==> 
+          is_serialized_certify_key_output hres w /\
+          struct_has_pubkey_and_cert hres pk c)
+{
+  let res = write_certify_key_output pubkey cert;
+  let sz = serialize_certifykeyoutputargs' _ out;
+  destruct_certifykeyoutputargs res _ pubkey cert p q pk c;
+  if (sz = 0sz) {
+     false
+  }
+  else {
+    true
+  }
+}
